## Test for whether an interpreter is using normal or applicative order.
```
(define (p) (p))
(define (test x y)
  (if (= x 0) 0 y))
```

Then 
```
(test 0 (p))
```

### Normal Order

The normal order follows the "expand-and-reduce" rule.

```
=> (test 0 (p))
=> (if (= 0 0) 0 (p)))
```

An interpreter using normal-order to evaluate the above expression will return a zero.
This is because the interpreter will fully expand the function before trying to evaluate it. Therefore, the `if` statement is carried out and the function p isn't called.

### Applicative order

The applicative order follows the "evaluate-and-reduce" rule.
An interpreter using applicative-order to evaluate the above expression will not return(stack overflow).
This is because it will try to evaluate what `(p)` is before passing it into the `test` function and `p`
is a function that calls itself (The scheme interpreter uses applicative-order so the function doesn't return).

```
=> (test 0 (p))
=> (test 0 (p))
=> (test 0 (p))
=> (test 0 (p))
=> (test 0 (p))
```

You get the idea.